correct cons and provide API

Cslib/Foundations/Data/StackTape.lean
@@ -31,52 +31,127 @@ namespace Turing
 List of `Option` values that don't end with `none`
 -/
 structure StackTape (α : Type) where
-  (asList : List (Option α))
+  (toList : List (Option α))
   -- The list can be empty (i.e. `none`),
   -- but if it is not empty, the last element is not (`some`) `none`
-  (h : asList.getLast? ≠ some none)
+  (toList_getLast?_ne_some_none : toList.getLast? ≠ some none)
 
-def StackTape.empty {α} : StackTape α := { asList := [], h := by simp }
+/-- The empty `StackTape` -/
+def StackTape.empty {α} : StackTape α := ⟨[], by simp⟩
 
-def StackTape.map_some {α} (l : List α) : StackTape α := { asList := l.map some, h := by simp }
+/-- Create a `StackTape` from a list by mapping all elements to `some` -/
+def StackTape.map_some {α} (l : List α) : StackTape α := ⟨l.map some, by simp⟩
 
 instance {α : Type} : Inhabited (StackTape α) where
   default := StackTape.empty
 
-def StackTape.length {α} (l : StackTape α) : ℕ := l.asList.length
+/-- The length of the `StackTape` is the number of elements up to the last non-`none` element -/
+def StackTape.length {α} (l : StackTape α) : ℕ := l.toList.length
 
-def StackTape.cons {α} : Option α -> StackTape α -> StackTape α
-| none, l => { asList := [], h := by simp }
-| some a, l => {
-    asList := some a :: l.asList,
-    h := by
-      cases hl : l.asList with
+/-- Prepend an `Option` to the `StackTape` -/
+def StackTape.cons {α} (x : Option α) (xs : StackTape α) : StackTape α :=
+  match x, xs with
+  | none, ⟨[], _⟩ => ⟨[], by simp⟩
+  | none, ⟨hd :: tl, hl⟩ => ⟨none :: hd :: tl, by simp only [List.getLast?_cons_cons]; exact hl⟩
+  | some a, ⟨l, hl⟩ => ⟨some a :: l, by
+      cases hl' : l with
       | nil => simp
       | cons hd tl =>
         simp only [List.getLast?_cons_cons]
-        rw [← hl]
-        exact l.h
-       }
+        exact ne_of_eq_of_ne (congrArg List.getLast? (id (Eq.symm hl'))) hl⟩
 
+/-- Remove the first element of the `StackTape`, returning the rest -/
 def StackTape.tail {α} (l : StackTape α) : StackTape α :=
-  match hl : l.asList with
+  match hl : l.toList with
   | [] => StackTape.empty
-  | hd :: t => { asList := t, h := by
-                  match t with
-                  | [] => simp
-                  | hd' :: t' =>
-                    have lh := l.h
-                    rw [hl] at lh
-                    simp only [List.getLast?_cons_cons] at lh
-                    have := l.h
-                    rw [hl, List.getLast?_cons_cons] at this
-                    exact this
-  }
+  | hd :: t => ⟨t, by
+      match t with
+      | [] => simp
+      | hd' :: t' =>
+        have lh := l.toList_getLast?_ne_some_none
+        rw [hl] at lh
+        simp only [List.getLast?_cons_cons] at lh
+        have := l.toList_getLast?_ne_some_none
+        rw [hl, List.getLast?_cons_cons] at this
+        exact this⟩
 
+/-- Get the first element of the `StackTape`. -/
 def StackTape.head {α} (l : StackTape α) : Option α :=
-  match l.asList with
+  match l.toList with
   | [] => none
   | h :: _ => h
+
+lemma StackTape.eq_iff {α} (l1 l2 : StackTape α) :
+    l1 = l2 ↔ l1.head = l2.head ∧ l1.tail = l2.tail := by
+  constructor
+  · intro h
+    rw [h]
+    simp
+  · intro ⟨hhead, htail⟩
+    cases l1 with | mk as1 h1 =>
+    cases l2 with | mk as2 h2 =>
+    simp only [mk.injEq]
+    cases as1 with
+    | nil =>
+      cases as2 with
+      | nil => rfl
+      | cons hd2 tl2 =>
+        simp only [head] at hhead
+        simp only [tail, empty, mk.injEq] at htail
+        subst htail hhead
+        simp at h2
+    | cons hd1 tl1 =>
+      cases as2 with
+      | nil =>
+        simp only [head] at hhead
+        simp only [tail, empty, mk.injEq] at htail
+        subst htail hhead
+        simp at h1
+      | cons hd2 tl2 =>
+        simp only [head] at hhead
+        simp only [tail, mk.injEq] at htail
+        rw [hhead, htail]
+
+@[simp]
+lemma StackTape.head_cons {α} (o : Option α) (l : StackTape α) :
+    (StackTape.cons o l).head = o := by
+  cases o with
+  | none =>
+    cases l with | mk toList hl =>
+    cases toList with
+    | nil => simp [cons, head]
+    | cons hd tl => simp [cons, head]
+  | some a => simp [cons, head]
+
+@[simp]
+lemma StackTape.tail_cons {α} (o : Option α) (l : StackTape α) :
+    (StackTape.cons o l).tail = l := by
+  cases o with
+  | none =>
+    cases l with | mk toList h =>
+    cases toList with
+    | nil => simp [cons, tail, empty]
+    | cons hd tl => simp [cons, tail]
+  | some a =>
+    simp only [cons]
+    unfold tail
+    simp only
+
+@[simp]
+lemma StackTape.cons_head_tail {α} (l : StackTape α) :
+    StackTape.cons (l.head) (l.tail) = l := by
+  cases l with | mk toList h =>
+  cases toList with
+  | nil => simp [head, tail, cons, empty]
+  | cons hd tl =>
+    simp only [head, tail]
+    cases hd with
+    | none =>
+      cases tl with
+      | nil => simp at h
+      | cons hd' tl' => simp [cons]
+    | some a =>
+      simp only [cons]
 
 lemma StackTape.length_tail_le {α} (l : StackTape α) : l.tail.length ≤ l.length := by
   unfold tail length
@@ -84,8 +159,12 @@ lemma StackTape.length_tail_le {α} (l : StackTape α) : l.tail.length ≤ l.len
   · simp [empty]
   · next heq => simp [heq]
 
-lemma StackTape.length_cons_none {α} (l : StackTape α) : (StackTape.cons none l).length = 0 := by
-  simp [cons, length]
+lemma StackTape.length_cons_none {α} (l : StackTape α) :
+    (StackTape.cons none l).length = l.length + if l.length = 0 then 0 else 1 := by
+  cases l with | mk toList h =>
+  cases toList with
+  | nil => simp [cons, length]
+  | cons hd tl => simp [cons, length]
 
 lemma StackTape.length_cons_some {α} (a : α) (l : StackTape α) :
     (StackTape.cons (some a) l).length = l.length + 1 := by
@@ -94,7 +173,9 @@ lemma StackTape.length_cons_some {α} (a : α) (l : StackTape α) :
 lemma StackTape.length_cons_le {α} (o : Option α) (l : StackTape α) :
     (StackTape.cons o l).length ≤ l.length + 1 := by
   cases o with
-  | none => simp [length_cons_none]
+  | none =>
+    simp only [length_cons_none]
+    split <;> omega
   | some a => simp [length_cons_some]
 
 lemma StackTape.length_map_some {α} (l : List α) : (StackTape.map_some l).length = l.length := by
